src/Utils2.fsti
@@ -1,7 +1,9 @@
 module Utils2
 
+module US = FStar.SizeT
 module U64 = FStar.UInt64
 module U32 = FStar.UInt32
+module FU = FStar.UInt
 
 open Steel.Effect.Atomic
 open Steel.Effect
@@ -9,8 +11,23 @@ open Steel.Reference
 module A = Steel.Array
 
 
+
 let array = Steel.ST.Array.array
 let ptr = Steel.ST.Array.ptr
+
+// 1) ptrdiff
+// 2) ffs64/ffz64
+val ffs64 (x: U64.t)
+  : Pure US.t
+  (requires U64.v x > 0)
+  (ensures fun r ->
+    US.v r < 64 /\
+    FU.nth (U64.v x) (U64.n - US.v r - 1) = false
+  )
+
+unfold let same_base_array (#a: Type) (arr1 arr2: array a)
+  =
+  A.base (A.ptr_of arr1) == A.base (A.ptr_of arr2)
 
 unfold let slab_metadata = r:array U64.t{A.length r = 4}
 
@@ -47,3 +64,34 @@ let nb_slots_correct
   (requires U32.v pos < U32.v (nb_slots size_class))
   (ensures U32.v (U32.mul pos size_class) <= U32.v page_size)
   = ()
+
+open FStar.Mul
+let lemma_div (x y z: nat)
+  : Lemma
+  (requires
+    x = y * z /\
+    z > 0
+  )
+  (ensures
+    x / z = y
+  )
+  =
+  FStar.Math.Lemmas.lemma_mod_plus 0 y z;
+  assert ((y * z) % z = 0)
+
+let array_to_bv_slice
+  (#n: nat)
+  (s0: Seq.lseq U64.t n)
+  (i: nat)
+  : Lemma
+  (requires
+    i < n
+  )
+  (ensures (
+    let bm0 = Bitmap4.array_to_bv2 s0 in
+    let x = Seq.index s0 i in
+    Seq.slice bm0 (i*64) ((i+1)*64)
+    =
+    FU.to_vec #64 (U64.v x)))
+  =
+  Bitmap4.array_to_bv_lemma_upd_set_aux4 s0 (i*64)
